src/Lean/Compiler/Util.lean
@@ -65,9 +65,9 @@ def mkEagerLambdaLiftingName (n : Name) (idx : Nat) : Name :=
 
 @[export lean_is_eager_lambda_lifting_name]
 def isEagerLambdaLiftingName : Name → Bool
-  | Name.str p s _ => "_elambda".isPrefixOf s || isEagerLambdaLiftingName p
-  | Name.num p _ _ => isEagerLambdaLiftingName p
-  | _              => false
+  | .str p s => "_elambda".isPrefixOf s || isEagerLambdaLiftingName p
+  | .num p _ => isEagerLambdaLiftingName p
+  | _        => false
 
 /-- Return the name of new definitions in the a given declaration.
     Here we consider only declarations we generate code for.
@@ -97,7 +97,7 @@ def mkUnsafeRecName (declName : Name) : Name :=
 /-- Return `some _` if the given name was created using `mkUnsafeRecName` -/
 @[export lean_is_unsafe_rec_name]
 def isUnsafeRecName? : Name → Option Name
-  | Name.str n "_unsafe_rec" _ => some n
+  | .str n "_unsafe_rec" => some n
   | _ => none
 
 end Compiler
