src/Lean/Message.lean
@@ -130,7 +130,7 @@ partial def formatAux : NamingContext → Option MessageDataContext → MessageD
   | nCtx, ctx,       tagged t d               =>
     /- Messages starting a trace context have their tags postfixed with `_traceCtx` so that
     we can detect them later. Here, we do so in order to print the trace context class. -/
-    if let Name.str cls "_traceCtx" _ := t then do
+    if let .str cls "_traceCtx" := t then do
       let d₁ ← formatAux nCtx ctx d
       return f!"[{cls}] {d₁}"
     else
