src/Lean/Meta/ReduceEval.lean
@@ -44,11 +44,11 @@ private partial def evalName (e : Expr) : MetaM Name := do
   let Expr.const c _ _ ← pure e.getAppFn | throwFailedToEval e
   let nargs := e.getAppNumArgs
   if      c == ``Lean.Name.anonymous && nargs == 0 then pure Name.anonymous
-  else if c == ``Lean.Name.str && nargs == 3 then do
+  else if c == ``Lean.Name.str && nargs == 2 then do
     let n ← evalName $ e.getArg! 0
     let s ← reduceEval $ e.getArg! 1
     pure $ Name.mkStr n s
-  else if c == ``Lean.Name.num && nargs == 3 then do
+  else if c == ``Lean.Name.num && nargs == 2 then do
     let n ← evalName $ e.getArg! 0
     let u ← reduceEval $ e.getArg! 1
     pure $ Name.mkNum n u
